adapt u64 in the same way as u32

Clean/Types/U64.lean
@@ -35,11 +35,11 @@ instance (T: Type) [Repr T] : Repr (U64 T) where
   reprPrec x _ := "⟨" ++ repr x.x0 ++ ", " ++ repr x.x1 ++ ", " ++ repr x.x2 ++ ", " ++ repr x.x3 ++ ", " ++ repr x.x4 ++ ", " ++ repr x.x5 ++ ", " ++ repr x.x6 ++ ", " ++ repr x.x7 ++ "⟩"
 
 namespace U64
+def to_limbs {F} (x : U64 F) : Vector F 8 := to_elements x
+def from_limbs {F} (v : Vector F 8) : U64 F := from_elements v
+
 def map {α β : Type} (x : U64 α) (f : α → β) : U64 β :=
   ⟨ f x.x0, f x.x1, f x.x2, f x.x3, f x.x4, f x.x5, f x.x6, f x.x7 ⟩
-
-lemma to_elements_map {α β : Type} (x : U64 α) (f : α → β) :
-  to_elements (map x f) = (to_elements x).map f := rfl
 
 def vals (x : U64 (F p)) : U64 ℕ := x.map ZMod.val
 
@@ -313,13 +313,23 @@ lemma from_byte_is_normalized {x : Fin 256} : (from_byte x).is_normalized (p:=p)
   repeat linarith [x.is_lt, p_large_enough.elim]
 
 namespace ByteVector
--- results about U64 when viewed as a vector of bytes, via `to_elements` and `from_elements`
+-- results about U64 when viewed as a vector of bytes, via `to_limbs` and `from_limbs`
+
+theorem from_limbs_to_limbs {F} (x : U64 F) :
+    U64.from_limbs x.to_limbs = x := rfl
+
+theorem to_limbs_from_limbs {F} (v : Vector F 8) :
+    (U64.from_limbs v).to_limbs = v := ProvableType.to_elements_from_elements ..
+
+theorem ext_iff {F} {x y : U64 F} :
+    x = y ↔ ∀ i (_ : i < 8), x.to_limbs[i] = y.to_limbs[i] := by
+  simp only [U64.to_limbs, ProvableType.ext_iff, size]
 
 omit [Fact (Nat.Prime p)] p_large_enough in
 theorem is_normalized_iff {x : U64 (F p)} :
-    x.is_normalized ↔ ∀ i (_ : i < 8), (to_elements x)[i].val < 256 := by
+    x.is_normalized ↔ ∀ i (_ : i < 8), x.to_limbs[i].val < 256 := by
   rcases x with ⟨ x0, x1, x2, x3, x4, x5, x6, x7 ⟩
-  simp only [is_normalized, to_elements, size, Vector.getElem_mk, List.getElem_toArray]
+  simp only [to_limbs, is_normalized, to_elements, size, Vector.getElem_mk, List.getElem_toArray]
   constructor
   · intro h i hi
     repeat (rcases hi with _ | hi; try simp [*, size])
@@ -335,5 +345,15 @@ theorem is_normalized_iff {x : U64 (F p)} :
     simp only [List.getElem_cons_zero, List.getElem_cons_succ] at h0 h1 h2 h3 h4 h5 h6 h7
     simp_all
 
+lemma to_limbs_map {α β : Type} (x : U64 α) (f : α → β) :
+  to_limbs (map x f) = (to_limbs x).map f := rfl
+
+lemma getElem_eval_to_limbs {F} [Field F] {env : Environment F} {x : U64 (Expression F)} {i : ℕ} (hi : i < 8) :
+    Expression.eval env x.to_limbs[i] = (eval env x).to_limbs[i] := by
+  simp only [to_limbs, eval, size, to_vars, ProvableType.to_elements_from_elements, Vector.getElem_map]
+
+lemma eval_from_limbs {F} [Field F] {env : Environment F} {v : Vector (Expression F) 8} :
+    eval env (U64.from_limbs v) = .from_limbs (v.map env) := by
+  simp only [U64.from_limbs, ProvableType.eval_from_elements]
 end ByteVector
 end U64
